LeanVerus/sst/exp_rep.lean
@@ -11,7 +11,7 @@ variable (tenv : typ_env)  (dom_aux : ClosedTyp → Type)
 def val_vars tenv (Γ: context) dom_aux :=  (i : Nat) → (_ : i < Γ.length) → typ_interp tenv dom_aux Γ[i]
 
 noncomputable
-def exp_rep Γ tenv (venv: val_vars tenv Γ dom_aux) (t : Typ) (e : Exp) (hty : Γ ⊢.{u} e : t): typ_interp tenv dom_aux t:=
+def exp_rep Γ tenv (venv: val_vars tenv Γ dom_aux) (t : Typ) (e : Exp) (hty : Γ ⊢ e : t): typ_interp tenv dom_aux t:=
   match e with
   | .Const c =>
     match c with
@@ -46,16 +46,38 @@ def exp_rep Γ tenv (venv: val_vars tenv Γ dom_aux) (t : Typ) (e : Exp) (hty : 
 
   | .Unaryr op arg =>
     match op with
+    | .HasType t' =>
+      cast_typ_interp (ty_hasType_inv arg t' t hty).symm (cast interp_bool.symm (Γ ⊢ arg : t'))
     | .Box t' => sorry
     | .Unbox t' => sorry
     | .IsVariant dt var => sorry
     | .Proj field => sorry
-    | .HasType t' =>
-      cast_typ_interp (ty_hasType_inv arg t' t hty).symm (cast interp_bool.symm (Γ ⊢.{u} arg : t'))
 
-  | .Unary op arg => sorry
+  | .Unary op arg =>
+    match op with
+    | .Not =>
+      exp_rep Γ tenv venv t arg (ty_not_inv arg hty).2
+    | .FloatToBits =>
+      match arg with
+      | _ => sorry
+
+      -- match (ty_floatToBits_inv arg hty) with
+      -- | Or.inl hl => sorry
+      -- | Or.inr hr => sorry
+    | .BitNot (width : Option Nat) => sorry
+    | .Clip (range : IntRange) (truncate : Bool) => sorry
 
 
+  | .Binary (op : BinaryOp) (arg₁ : Exp) (arg₂ : Exp)=> sorry
+  | .If c b₁ b₂ => sorry
+  | .Let (tys : List Typ) (es : List Exp) (body : Exp) => sorry
+  | .Quant (q : Quant) (var : Typ) (body : Exp) => sorry
+  | .TupleCtor (size : Nat) (data : List Exp) => sorry
 
-  | _ => sorry
+
+  | .Call (fn : CallFun) (typs : List Typ) (exps : List Exp) (ret : Typ) => sorry
+  | .CallLambda (lam : Exp) (arg : Exp) => sorry
+  | .StructCtor (dt : Ident) (fields : List (String × Exp)) => sorry
+  | .Lambda (var : Typ) (exp : Exp) => sorry
+
 termination_by sizeOf e
